Do substitution when opening

src/constr-dot/ConstrLang.v
@@ -13,18 +13,12 @@ Set Implicit Arguments.
 Require Import TLC.LibLN.
 Require Import String.
 
-Require Import Definitions RecordAndInertTypes.
-
-
-Inductive tvar : Set :=
-  | tvar_b : nat -> tvar
-  | tvar_f : var -> tvar.
+Require Import Definitions RecordAndInertTypes Decompose.
 
 
 Inductive ctyp : Set :=
-  | ctyp_tvar : tvar -> ctyp
+  | ctyp_tvar_b : nat -> ctyp
   | ctyp_typ : typ -> ctyp.
-
 
 Inductive constr : Set :=
 | constr_true : constr
@@ -51,179 +45,111 @@ Notation "C '⋎' D" := (constr_or C D) (at level 30).
 (** - type existence constraint *)
 Notation "'∃t' C" := (constr_exists_typ C) (at level 30).
 
+(** - typing constraint *)
 Notation "x '⦂' T" := (constr_typ x T) (at level 29).
 
+(** - subtyping constraint *)
 Notation "S '<⦂' T" := (constr_sub S T) (at level 29).
 
-Definition open_rec_tvar (k : nat) (u : var) (tv : tvar) : tvar :=
-  match tv with
-  | tvar_b i => If k = i then tvar_f u else tvar_b i
-  | tvar_f x => tvar_f x
-  end.
 
-
-Definition open_rec_ctyp (k : nat) (u : var) (T : ctyp) : ctyp :=
+Definition open_rec_ctyp (k : nat) (S : typ) (T : ctyp) : ctyp :=
   match T with
-  | ctyp_tvar tv => ctyp_tvar (open_rec_tvar k u tv)
+  | ctyp_tvar_b i => If k = i then ctyp_typ S else ctyp_tvar_b i
   | ctyp_typ T0 => ctyp_typ T0
   end.
 
-Fixpoint open_rec_constr (k : nat) (u : var) (C : constr) : constr :=
+Fixpoint open_rec_constr (k : nat) (T : typ) (C : constr) : constr :=
   match C with
   | constr_true => constr_true
   | constr_false => constr_false
-  | constr_and C1 C2 => constr_and (open_rec_constr k u C1) (open_rec_constr k u C2)
-  | constr_or C1 C2 => constr_or (open_rec_constr k u C1) (open_rec_constr k u C2)
-  | constr_exists_typ C => constr_exists_typ (open_rec_constr (S k) u C)
-  | constr_sub T1 T2 => constr_sub (open_rec_ctyp k u T1) (open_rec_ctyp k u T2)
-  | constr_typ t T => constr_typ t (open_rec_ctyp k u T)
+  | constr_and C1 C2 => constr_and (open_rec_constr k T C1) (open_rec_constr k T C2)
+  | constr_or C1 C2 => constr_or (open_rec_constr k T C1) (open_rec_constr k T C2)
+  | constr_exists_typ C => constr_exists_typ (open_rec_constr (S k) T C)
+  | constr_sub T1 T2 => constr_sub (open_rec_ctyp k T T1) (open_rec_ctyp k T T2)
+  | constr_typ t T0 => constr_typ t (open_rec_ctyp k T T0)
   end.
 
 
-Definition open_tvar (u : var) (tv : tvar) : tvar := open_rec_tvar 0 u tv.
-Definition open_ctyp (u : var) (T : ctyp) : ctyp := open_rec_ctyp 0 u T.
-Definition open_constr (u : var) (C : constr) : constr := open_rec_constr 0 u C.
-
-
-Fixpoint fv_tvar (tv : tvar) :=
-  match tv with
-  | tvar_b i => \{}
-  | tvar_f x => \{x}
-  end.
-
-
-Fixpoint fv_ctyp (T : ctyp) :=
-  match T with
-  | ctyp_tvar tv => fv_tvar tv
-  | ctyp_typ T => \{}
-  end.
+Definition open_ctyp (S : typ) (T : ctyp) : ctyp := open_rec_ctyp 0 S T.
+Definition open_constr (T : typ) (C : constr) : constr := open_rec_constr 0 T C.
 
 
 Inductive ctyp_lc : ctyp -> Prop :=
-
 | ctyp_typ_lc : forall T, ctyp_lc (ctyp_typ T)
-
-| ctyp_tvar_f_lc : forall x, ctyp_lc (ctyp_tvar (tvar_f x))
-
 .
 
 
 Inductive constr_lc : constr -> Prop :=
-
 | constr_true_lc: constr_lc ⊤
-
 | constr_false_lc: constr_lc ⊥
-
 | constr_and_lc : forall C1 C2,
     constr_lc C1 ->
     constr_lc C2 ->
     constr_lc (C1 ⋏ C2)
-
 | constr_or_lc : forall C1 C2,
     constr_lc C1 ->
     constr_lc C2 ->
     constr_lc (C1 ⋎ C2)
-
 | constr_exists_typ_lc : forall L C,
     (forall x, x \notin L -> constr_lc (open_constr x C)) ->
     constr_lc (∃t C)
-
 | constr_sub_lc : forall S T,
     ctyp_lc S ->
     ctyp_lc T ->
     constr_lc (S <⦂ T)
-
 | constr_typ_lc : forall t T,
     ctyp_lc T ->
     constr_lc (t ⦂ T)
-
 .
 
-Lemma lc_ctyp_open_unchanged : forall u T,
+Lemma lc_ctyp_open_unchanged : forall S T,
     ctyp_lc T ->
-    open_ctyp u T = T.
+    open_ctyp S T = T.
 Proof.
   introv Hc.
   induction Hc; eauto.
 Qed.
 
-Definition tmap := env typ.
+Reserved Notation "G '⊧' C" (at level 40).
 
-Inductive map_ctyp : tmap -> ctyp -> typ -> Prop :=
+Inductive satisfy_constr : ctx -> constr -> Prop :=
 
-  | map_ctyp_tvar : forall tm a T,
-      binds a T tm ->
-      map_ctyp tm (ctyp_tvar (tvar_f a)) T
+| sat_true : forall G,
+    G ⊧ ⊤
 
-  | map_ctyp_typ : forall tm T,
-      map_ctyp tm (ctyp_typ T) T
+| sat_and : forall G C1 C2,
+    G ⊧ C1 ->
+    G ⊧ C2 ->
+    G ⊧ C1 ⋏ C2
 
-.
+| sat_or1 : forall G C1 C2,
+    G ⊧ C1 ->
+    G ⊧ C1 ⋎ C2
 
-Lemma map_bound_tvar : forall tm x T T',
-    binds x T tm ->
-    map_ctyp tm (ctyp_tvar (tvar_f x)) T' ->
-    T = T'.
-Proof.
-  introv Hb Hm. inversion Hm; subst.
-  eapply binds_functional.
-  - apply Hb.
-  - apply H1.
-Qed.
+| sat_or2 : forall G C1 C2,
+    G ⊧ C2 ->
+    G ⊧ C1 ⋎ C2
 
+| sat_exists_typ : forall G T C,
+    G ⊧ open_constr T C ->
+    G ⊧ (∃t C)
 
-Lemma map_ctyp_fresh_extend : forall tm X T S S',
-    map_ctyp tm S S' ->
-    X \notin fv_ctyp S ->
-    map_ctyp (tm & X ~ T) S S'.
-Proof.
-  introv Hm Hn.
-  inversion Hm; subst.
-  - apply* map_ctyp_tvar.
+| sat_typ : forall G t T,
+    G ⊢ t : T ->
+    G ⊧ t ⦂ ctyp_typ T
 
+| sat_sub : forall G S T,
+    G ⊢ S <: T ->
+    G ⊧ ctyp_typ S <⦂ ctyp_typ T
 
-Inductive satisfy_constr : tmap -> ctx -> constr -> Prop :=
-
-| sat_true : forall tm G,
-    satisfy_constr tm G constr_true
-
-| sat_and : forall tm G C1 C2,
-    satisfy_constr tm G C1 ->
-    satisfy_constr tm G C2 ->
-    satisfy_constr tm G (C1 ⋏ C2)
-
-| sat_or1 : forall tm G C1 C2,
-    satisfy_constr tm G C1 ->
-    satisfy_constr tm G (C1 ⋎ C2)
-
-| sat_or2 : forall tm G C1 C2,
-    satisfy_constr tm G C2 ->
-    satisfy_constr tm G (C1 ⋎ C2)
-
-| sat_exists_typ : forall tm G T L C,
-    (forall X, X \notin L ->
-      satisfy_constr (tm & X ~ T) G (open_constr X C)) ->
-    satisfy_constr tm G (∃t C)
-
-| sat_typ : forall tm G t T T',
-    map_ctyp tm T T' ->
-    G ⊢ t : T' ->
-    satisfy_constr tm G (t ⦂ T)
-
-| sat_sub : forall tm G S S' T T',
-    map_ctyp tm S S' ->
-    map_ctyp tm T T' ->
-    G ⊢ S' <: T' ->
-    satisfy_constr tm G (constr_sub S T)
-
-.
+where "G '⊧' C" := (satisfy_constr G C).
 
 Hint Constructors satisfy_constr constr.
 
 Definition constr_entail (C1 C2 : constr) :=
-  forall tm G,
+  forall G,
     inert G ->
-    satisfy_constr tm G C1 -> satisfy_constr tm G C2.
+    satisfy_constr G C1 -> satisfy_constr G C2.
 
 
 Notation "C '⊩' D" := (constr_entail C D) (at level 50).
@@ -263,36 +189,42 @@ Theorem ent_and_left : forall C D,
     C ⋏ D ⊩ C.
 Proof. introe. inversion H; subst. eauto. Qed.
 
-Definition ctyp_b (i : nat) := ctyp_tvar (tvar_b i).
-
-(** ∃ U. (S <: U ⋏ U <: T) ⊩ S <: T *)
+(** If U is fresh for S and T, then
+    ∃ U. (S <: U ⋏ U <: T) ⊩ S <: T
+ *)
 Theorem ent_sub_trans : forall S T,
     ctyp_lc S -> ctyp_lc T ->
-    ∃t (S <⦂ (ctyp_b 0) ⋏ (ctyp_b 0) <⦂ T) ⊩ S <⦂ T.
+    ∃t (S <⦂ (ctyp_tvar_b 0) ⋏ (ctyp_tvar_b 0) <⦂ T) ⊩ S <⦂ T.
 Proof.
   introv Hs Ht.
   introe. inversion H; subst.
-  unfold open_constr in H4. simpl in H4.
+  unfold open_constr in H3. simpl in H3.
   case_if. clear C.
-  pick_fresh_gen (L \u fv_ctyp S \u fv_ctyp T) X.
-  specialize (H4 X). assert (X \notin L) as Hnl. { eauto. }
-  specialize (H4 Hnl).
-  inversion H4; subst.
-  pose proof (lc_ctyp_open_unchanged X Hs) as Hsu.
-  unfold open_ctyp in Hsu. rewrite -> Hsu in H6.
-  pose proof (lc_ctyp_open_unchanged X Ht) as Hst.
-  unfold open_ctyp in Hst. rewrite -> Hst in H7.
-  inversion H6; subst.
-  inversion H7; subst.
-  assert (T0 = T') as Heq1.
-  {
-    apply* map_bound_tvar.
-  }
-  assert (T0 = S'0) as Heq2.
-  {
-    apply* map_bound_tvar.
-  }
-  subst.
-  apply sat_sub with (S' := S') (T' := T'0).
-  - 
+  pose proof (lc_ctyp_open_unchanged T0 Hs) as Hsu.
+  unfold open_ctyp in Hsu. rewrite -> Hsu in H3.
+  pose proof (lc_ctyp_open_unchanged T0 Ht) as Hst.
+  unfold open_ctyp in Hst. rewrite -> Hst in H3.
+  clear Hsu Hst.
+  inversion H3; subst. clear H3.
+  inversion H5; clear H5; subst.
+  inversion H6; clear H6; subst.
+  apply* sat_sub.
+Qed.
+
+Theorem ent_and_true : forall C,
+    C ⋏ ⊤ ⊩ C.
+Proof.
+  introv. introe.
+  inversion H; subst; clear H. auto.
+Qed.
+
+Theorem ent_inv_subtyp_typ : forall A S1 T1 S2 T2,
+    ctyp_typ (typ_rcd (dec_typ A S1 T1)) <⦂ ctyp_typ (typ_rcd (dec_typ A S2 T2)) ⊩
+        ctyp_typ S2 <⦂ ctyp_typ S1 ⋏ ctyp_typ T1 <⦂ ctyp_typ T2.
+Proof.
+  introv. introe.
+  inversion H; subst; clear H.
+  apply invert_subtyp_typ in H3 as [Hs1 Hs2]; try assumption.
+  constructor; constructor; auto.
+Qed.
 
